src/program_proof/memkv/memkv_shard_definitions.v
@@ -69,11 +69,6 @@ Definition PostShardConditionalPut Eo Ei γkv (key:u64) Q expv newv (rep:ShardRe
   ⌜rep.(SR_Err) ≠ 0⌝ ∗ (PreShardConditionalPut Eo Ei γkv key Q expv newv) ∨ ⌜rep.(SR_Err) = 0⌝ ∗ Q rep.(SR_Success).
 
 
-Definition own_shard γkv sid (m:gmap u64 (list u8)) : iProp Σ :=
-  [∗ set] k ∈ (fin_to_set u64), ⌜shardOfC k ≠ sid⌝ ∨
-                                kvptsto γkv k (default [] (m !! k))
-.
-
 Definition is_shard_server_pre (ρ:u64 -d> memkv_shard_names -d> iPropO Σ) : (u64 -d> memkv_shard_names -d> iPropO Σ) :=
   λ host γ,
   ("#His_rpc" ∷ is_RPCServer γ.(rpc_gn) ∗
