src/goose_lang/dist_adequacy.v
@@ -14,7 +14,7 @@ Theorem heap_dist_adequacy `{ffi_sem: ffi_semantics} `{!ffi_interp ffi} {Hffi_ad
         g φinv (HINITG: ffi_initgP g) (HINIT: ∀ σ, σ ∈ init_local_state <$> ebσs → ffi_initP σ.(world) g) :
   (∀ `{Hheap : !heap_globalG Σ} (cts : list (crashG Σ * heap_local_names)),
       ⊢
-        ffi_pre_global_start Σ (heap_preG_ffi) (heap_globalG_names) g ={⊤}=∗
+        ffi_pre_global_start Σ (heap_preG_ffi (heapPreG := heap_globalG_preG)) (heap_globalG_names) g ={⊤}=∗
         ([∗ list] i ↦ ct; σ ∈ cts; init_local_state <$> ebσs,
               let hG := heap_globalG_heapG Hheap (fst ct) (snd ct) in
               ffi_local_start (heapG_ffiG) σ.(world) g ∗ trace_frag σ.(trace) ∗ oracle_frag σ.(oracle)) ={⊤}=∗
@@ -116,7 +116,7 @@ Theorem heap_dist_adequacy_alt `{ffi_sem: ffi_semantics} `{!ffi_interp ffi} {Hff
         g φinv (HINITG: ffi_initgP g) (HINIT: ∀ σ, σ ∈ init_local_state <$> ebσs → ffi_initP σ.(world) g) :
   (∀ `{Hheap : !heap_globalG Σ},
       ⊢
-        ffi_pre_global_start Σ (heap_preG_ffi) (heap_globalG_names) g ={⊤}=∗
+        ffi_pre_global_start Σ (heap_preG_ffi (heapPreG := heap_globalG_preG)) (heap_globalG_names) g ={⊤}=∗
         ([∗ list] ebσ ∈ ebσs,
               let e := init_thread ebσ in
               let r := init_restart ebσ in
@@ -168,7 +168,7 @@ Theorem heap_dist_adequacy_failstop
         g φinv (HINITG: ffi_initgP g) (HINIT: ∀ σ, σ ∈ snd  <$> ebσs → ffi_initP σ.(world) g) :
   (∀ `{Hheap : !heap_globalG Σ},
       ⊢
-        ffi_pre_global_start Σ (heap_preG_ffi) (heap_globalG_names) g ={⊤}=∗
+        ffi_pre_global_start Σ (heap_preG_ffi (heapPreG := heap_globalG_preG)) (heap_globalG_names) g ={⊤}=∗
         ([∗ list] ebσ ∈ ebσs,
               let e := fst ebσ in
               let σ := snd ebσ in
