src/program_proof/memkv/closed.v
@@ -1,0 +1,64 @@
+From Perennial.algebra Require Import gen_heap_names.
+From Perennial.goose_lang Require Import lang notation typing lifting.
+From Perennial.goose_lang.lib Require Import map.impl list.impl list_slice.
+From Perennial.goose_lang Require Import prelude.
+From Perennial.goose_lang.ffi Require Import dist_ffi.
+From Perennial.goose_lang Require Import ffi.dist_prelude.
+From Goose.github_com.mit_pdos.gokv Require Import memkv.
+
+
+From Perennial.program_proof Require Import dist_prelude.
+From Perennial.program_proof.lockservice Require Export rpc.
+From Perennial.program_proof.memkv Require Export
+     memkv_shard_definitions memkv_shard_start_proof memkv_shard_make_proof memkv_shard_ghost_init.
+
+Definition shard_boot (host : u64) : expr :=
+  let: "s" := MakeMemKVShardServer #true in
+  MemKVShardServer__Start "s" #host.
+
+From Perennial.goose_lang Require Import adequacy recovery_adequacy dist_adequacy.
+
+Definition shardΣ := #[heapΣ; kvMapΣ; rpcΣ ShardReplyC; rpcregΣ].
+
+Lemma shard_boot1 (host : chan) σ (g : ffi_global_state) :
+  ffi_initgP g →
+  ffi_initP σ.(world) g →
+  (g : gmap chan (gset message)) !! host = Some (∅ : gset message) →
+  dist_adequate_failstop [(shard_boot host, σ)] g (λ _, True).
+Proof.
+  intros Hinit1 Hinit2 Hlookup.
+  eapply (heap_dist_adequacy_failstop (shardΣ)).
+  { assumption. }
+  { auto. }
+  intros Hheap. rewrite /=.
+  iIntros "(Hchan&_)".
+
+  (* Get out the channel for the server *)
+  iDestruct (big_sepM_lookup_acc with "Hchan") as "(Hg&_)"; first eassumption.
+  remember (uNSHARD) as uNSHARD' eqn:Heq_unSHARD'.
+  iMod (kvptsto_init uNSHARD') as (γkv) "(Hserver_shards&Hclients_ptstos)".
+  iMod (shard_server_ghost_init host γkv with "[$Hg]") as (γ Heq_kv) "(#Hdom&#Hsrv&Hsrv_rpc_ghost&Hsrv_cid)".
+
+  iModIntro.
+  iSplitR ""; last first.
+  { iMod (fupd_mask_subseteq ∅); eauto. }
+  iSplitR ""; last eauto.
+
+  iIntros (Hcrash local_names) "(_&?&?)".
+
+  iModIntro. iExists (λ _, True%I).
+  rewrite /shard_boot.
+  wp_bind (MakeMemKVShardServer #true).
+  wp_apply (wp_MakeMemKVShardServer with "[Hsrv_cid Hserver_shards Hsrv_rpc_ghost]").
+  { iSplitL "".
+    { rewrite is_shard_server_unfold. iNamed "Hsrv". iFrame "#". }
+    iClear "Hsrv". iFrame "Hsrv_rpc_ghost".
+    rewrite -Heq_unSHARD' Heq_kv. iFrame "Hserver_shards".
+    eauto. }
+  iIntros (s) "His_server".
+  wp_pures.
+  wp_apply (wp_MemKVShardServer__Start with "[] [] [$His_server]").
+  { iExactEq "Hdom". rewrite //=. f_equal. set_solver. }
+  { admit. }
+  eauto.
+Abort.
